SlowTest/DiffLogic-Test/seq_Dafny.dfy
@@ -1,5 +1,17 @@
 
-method S(a: seq<bool>)
+function method Dec(a: int, b: int) : int
+lemma Props_dec (sum: int, a: int, b: int)
+    requires a > b
+    ensures Dec(sum, a) < Dec(sum, b)
+
+lemma Props_dec_one (sum: int)
+    ensures forall j :: Dec(sum, j + 1) < Dec(sum, j)
+
+lemma Props_dec_lower_bound (sum: int, x: int)
+    requires x <= sum
+    ensures 0 <= Dec(sum, x)
+
+method S1()
 {
     var a: seq<bool>;
     var len: int := |a|;
@@ -8,13 +20,12 @@ method S(a: seq<bool>)
         invariant |a| == len
         invariant 0 <= i <= len
         invariant forall j :: 0 <= j < i ==> a[j]
-        decreases len - i
+        decreases Dec(len, i)
     {
         a := a[i := true];
-        assert (len - (i + 1) < len - i);
-        assert (i < len ==> i + 1 <= len);
-        // assume ()
-        assume (forall j: int :: i == j ==> a[j]);
+        // Props_dec(len, i + 1, i); // Error: decreases expression might not decrease
+        Props_dec_one (len); // works
+        Props_dec_lower_bound(len, i);
         i := i + 1;
     }
     assert (forall j: int :: 0 <= j < len ==> a[j]);
